lib/Lib.Buffer.fsti
@@ -18,7 +18,7 @@ module Seq = Lib.Sequence
 module ByteSeq = Lib.ByteSequence
 module Loop = Lib.LoopCombinators
 
-#set-options "--z3rlimit 15"
+#set-options "--z3rlimit 20 --max_fuel 0 --max_ifuel 1"
 
 type buftype =
   | MUT
@@ -41,7 +41,6 @@ let length (#t:buftype) (#a:Type0) (b:buffer_t t a) =
   | MUT -> B.length (b <: buffer a)
   | IMMUT -> IB.length (b <: ibuffer a)
 
-
 inline_for_extraction
 let lbuffer_t (ty:buftype) (a:Type0) (len:size_t) =
   b:buffer_t ty a{length #ty #a b == v len}
@@ -59,6 +58,8 @@ let loc (#t:buftype) (#a:Type0) (b:buffer_t t a) : GTot B.loc =
   match t with
   | MUT -> B.loc_buffer (b <: buffer a)
   | IMMUT -> B.loc_buffer (b <: ibuffer a)
+
+#set-options "--max_ifuel 0"
 
 let union (l1:B.loc) (l2:B.loc) : GTot B.loc = B.loc_union l1 l2
 let ( |+| ) (l1:B.loc) (l2:B.loc) : GTot B.loc = union l1 l2
@@ -129,8 +130,6 @@ let as_seq (#t:buftype) (#a:Type0) (#len:size_t) (h:HS.mem) (b:lbuffer_t t a len
   match t with
   | MUT -> B.as_seq h (b <: buffer a)
   | IMMUT -> IB.as_seq h (b <: ibuffer a)
-
-#reset-options "--z3rlimit 100"
 
 (** Ghostly get a sub-buffer of a buffer *)
 let gsub (#t:buftype) (#a:Type0) (#len:size_t) (b:lbuffer_t t a len)
@@ -347,6 +346,8 @@ val create:
     (requires fun h0 -> v len > 0)
     (ensures  fun h0 b h1 -> live h1 b /\ stack_allocated b h0 h1 (Seq.create (v len) init))
 
+#set-options "--max_fuel 1"
+
 (** Allocate a stack fixed-length mutable buffer initialized to a list *)
 inline_for_extraction noextract
 val createL:
@@ -366,6 +367,8 @@ val createL_global:
     (ensures  fun h0 b h1 -> global_allocated b h0 h1 (Seq.of_list init) /\
                           recallable b /\
                           witnessed b (Seq.of_list init))
+
+#set-options "--max_fuel 0"
 
 (** Recall the liveness and contents of a global immutable buffer *)
 inline_for_extraction noextract
@@ -907,6 +910,8 @@ val fill_blocks_:
       as_seq #_ #t h1 (gsub output (size 0) (n *! len)) == o)
 *)
 
+#set-options "--z3rlimit 150"
+
 (** Fills a buffer block by block using a function with an accumulator *)
 inline_for_extraction noextract
 val fill_blocks:
@@ -1054,8 +1059,6 @@ val mapi:
       modifies1 o h h1 /\
       as_seq h1 o == Seq.mapi (spec_f h0) (as_seq h i))
 
-
-#set-options "--z3rlimit 150 --max_fuel 1 --max_ifuel 1"
 inline_for_extraction noextract
 val map_blocks_multi:
     #t:buftype
