lib/Lib.ByteSequence.fsti
@@ -19,13 +19,13 @@ unfold inline_for_extraction let pub_bytes = bytes_l PUB
 unfold inline_for_extraction let pub_lbytes (len:size_nat) = lbytes_l PUB len
 
 (** Construct the equality mask for a pair of secret integer sequences *)
-val seq_eq_mask: #t:inttype{~(U1? t)} -> #len1:size_nat -> #len2:size_nat
-  -> b1:lseq (uint_t t SEC) len1
-  -> b2:lseq (uint_t t SEC) len2
+val seq_eq_mask: #t:inttype{~(S128? t)} -> #len1:size_nat -> #len2:size_nat
+  -> b1:lseq (int_t t SEC) len1
+  -> b2:lseq (int_t t SEC) len2
   -> len:size_nat{len <= len1 /\ len <= len2}
-  -> res:uint_t t SEC{
+  -> res:int_t t SEC{
       (sub b1 0 len == sub b2 0 len  ==> v res == v (ones t SEC)) /\
-      (sub b1 0 len =!= sub b2 0 len ==> v res == v (zeroes t SEC))}
+      (sub b1 0 len =!= sub b2 0 len ==> v res == v (zeros t SEC))}
 
 (** Compares two byte sequences and declassifies the result *)
 inline_for_extraction
@@ -39,11 +39,11 @@ let lbytes_empty: lbytes 0 = create 0 (u8 0)
 /// Conversions between natural numbers and sequences
 
 inline_for_extraction
-val nat_from_intseq_be: #t:inttype -> #l:secrecy_level -> b:seq (uint_t t l)
+val nat_from_intseq_be: #t:inttype{unsigned t} -> #l:secrecy_level -> b:seq (uint_t t l)
   -> n:nat{n < pow2 (length b * bits t)}
 
 inline_for_extraction
-val nat_from_intseq_le: #t:inttype -> #l:secrecy_level
+val nat_from_intseq_le: #t:inttype{unsigned t} -> #l:secrecy_level
   -> b:seq (uint_t t l) -> n:nat{n < pow2 (length b * bits t)}
 
 inline_for_extraction
@@ -53,11 +53,11 @@ inline_for_extraction
 val nat_from_bytes_le: #l:secrecy_level -> b:bytes_l l -> n:nat{n < pow2 (length b * 8)}
 
 inline_for_extraction
-val nat_to_intseq_be: #t:inttype -> #l:secrecy_level -> len:nat -> n:nat{n < pow2 (bits t * len)} ->
+val nat_to_intseq_be: #t:inttype{unsigned t} -> #l:secrecy_level -> len:nat -> n:nat{n < pow2 (bits t * len)} ->
   b:seq (uint_t t l){length b == len /\ n == nat_from_intseq_be b}
 
 inline_for_extraction
-val nat_to_intseq_le: #t:inttype -> #l:secrecy_level -> len:nat -> n:nat{n < pow2 (bits t * len)} ->
+val nat_to_intseq_le: #t:inttype{unsigned t} -> #l:secrecy_level -> len:nat -> n:nat{n < pow2 (bits t * len)} ->
   b:seq (uint_t t l){length b == len /\ n == nat_from_intseq_le b}
 
 inline_for_extraction
@@ -69,63 +69,63 @@ val nat_to_bytes_le: #l:secrecy_level -> len:nat -> n:nat{n < pow2 (8 * len)}
   -> b:bytes_l l{length b == len /\ n == nat_from_intseq_le #U8 b}
 
 inline_for_extraction
-val uint_to_bytes_le: #t:inttype -> #l:secrecy_level -> uint_t t l -> lbytes_l l (numbytes t)
+val uint_to_bytes_le: #t:inttype{unsigned t} -> #l:secrecy_level -> uint_t t l -> lbytes_l l (numbytes t)
 
-val index_uint_to_bytes_le: #t:inttype -> #l:secrecy_level -> u:uint_t t l
+val index_uint_to_bytes_le: #t:inttype{unsigned t} -> #l:secrecy_level -> u:uint_t t l
   -> Lemma
     (forall (i:nat{i < numbytes t}). index (uint_to_bytes_le #t #l u) i ==
-                              uint #U8 #l (uint_v u / pow2 (op_Multiply 8 i) % pow2 8))
+                              uint #U8 #l (v u / pow2 (op_Multiply 8 i) % pow2 8))
 
 inline_for_extraction
-val uint_to_bytes_be: #t:inttype -> #l:secrecy_level -> u:uint_t t l -> lbytes_l l (numbytes t)
+val uint_to_bytes_be: #t:inttype{unsigned t} -> #l:secrecy_level -> u:uint_t t l -> lbytes_l l (numbytes t)
 
 inline_for_extraction
-val uint_from_bytes_le: #t:inttype{~(t == U1)} -> #l:secrecy_level
+val uint_from_bytes_le: #t:inttype{unsigned t /\ ~(U1? t)} -> #l:secrecy_level
   -> b:lbytes_l l (numbytes t) -> uint_t t l
 
 inline_for_extraction
-val uint_from_bytes_be: #t:inttype{~(t == U1)} -> #l:secrecy_level
+val uint_from_bytes_be: #t:inttype{unsigned t /\ ~(U1? t)} -> #l:secrecy_level
   -> lbytes_l l (numbytes t) -> uint_t t l
 
 inline_for_extraction
-val uints_to_bytes_le: #t:inttype -> #l:secrecy_level -> #len:size_nat{len * numbytes t < pow2 32}
+val uints_to_bytes_le: #t:inttype{unsigned t} -> #l:secrecy_level -> #len:size_nat{len * numbytes t < pow2 32}
   -> lseq (uint_t t l) len -> lbytes_l l (len * numbytes t)
 
-val index_uints_to_bytes_le: #t:inttype -> #l:secrecy_level -> #len:size_nat{len * numbytes t < pow2 32}
+val index_uints_to_bytes_le: #t:inttype{unsigned t} -> #l:secrecy_level -> #len:size_nat{len * numbytes t < pow2 32}
   -> ul:lseq (uint_t t l) len -> i:nat{i < len * numbytes t}
   -> Lemma
     (index (uints_to_bytes_le #t #l #len ul) i == (uint_to_bytes_le ul.[i / numbytes t]).[i % numbytes t])
 
 inline_for_extraction
-val uints_to_bytes_be: #t:inttype -> #l:secrecy_level -> #len:size_nat{len * numbytes t < pow2 32}
+val uints_to_bytes_be: #t:inttype{unsigned t} -> #l:secrecy_level -> #len:size_nat{len * numbytes t < pow2 32}
   -> lseq (uint_t t l) len -> lbytes_l l (len * numbytes t)
 
 inline_for_extraction
-val uints_from_bytes_le: #t:inttype{~(t == U1)} -> #l:secrecy_level -> #len:size_nat{len * numbytes t < pow2 32}
+val uints_from_bytes_le: #t:inttype{unsigned t /\ ~(U1? t)} -> #l:secrecy_level -> #len:size_nat{len * numbytes t < pow2 32}
   -> lbytes_l l (len * numbytes t) -> lseq (uint_t t l) len
 
-val index_uints_from_bytes_le: #t:inttype{~(t == U1)} -> #l:secrecy_level -> #len:size_nat{len * numbytes t < pow2 32}
+val index_uints_from_bytes_le: #t:inttype{unsigned t /\ ~(U1? t)} -> #l:secrecy_level -> #len:size_nat{len * numbytes t < pow2 32}
   -> b:lbytes_l l (len * numbytes t) -> i:size_nat{i < len}
   -> Lemma
     (index (uints_from_bytes_le #t #l #len b) i == uint_from_bytes_le (sub b (i * numbytes t) (numbytes t)))
 
 inline_for_extraction
-val uints_from_bytes_be: #t:inttype{~(t == U1)} -> #l:secrecy_level -> #len:size_nat{len * numbytes t < pow2 32}
+val uints_from_bytes_be: #t:inttype{unsigned t /\ ~(U1? t)} -> #l:secrecy_level -> #len:size_nat{len * numbytes t < pow2 32}
   -> lbytes_l l (len * numbytes t) -> lseq (uint_t t l) len
 
 inline_for_extraction
-val uint_at_index_le: #t:inttype{~(t == U1)} -> #l:secrecy_level -> #len:size_nat{len * numbytes t < pow2 32}
+val uint_at_index_le: #t:inttype{unsigned t /\ ~(U1? t)} -> #l:secrecy_level -> #len:size_nat{len * numbytes t < pow2 32}
   -> b:lbytes_l l (len * numbytes t)
   -> idx:nat{idx < len}
   -> u:uint_t t l{u == (uints_from_bytes_le #t #l #len b).[idx]}
 
 inline_for_extraction
-val uint_at_index_be: #t:inttype{~(t == U1)} -> #l:secrecy_level -> #len:size_nat{len * numbytes t < pow2 32}
+val uint_at_index_be: #t:inttype{unsigned t /\ ~(U1? t)} -> #l:secrecy_level -> #len:size_nat{len * numbytes t < pow2 32}
   -> b:lbytes_l l (len * numbytes t)
   -> idx:nat{idx < len}
   -> u:uint_t t l{u == (uints_from_bytes_be #t #l #len b).[idx]}
 
-val nat_from_intseq_le_slice_lemma: #t:inttype -> #l:secrecy_level -> #len:size_nat
+val nat_from_intseq_le_slice_lemma: #t:inttype{unsigned t} -> #l:secrecy_level -> #len:size_nat
   -> b:lseq (uint_t t l) len -> i:nat{i <= len} ->
   Lemma (nat_from_intseq_le b == nat_from_intseq_le (Seq.slice b 0 i) + pow2 (i * bits t) * nat_from_intseq_le (Seq.slice b i len))
 
@@ -133,27 +133,23 @@ val nat_from_bytes_le_slice_lemma: #l:secrecy_level -> #len:size_nat
   -> b:lbytes_l l len -> i:nat{i <= len} ->
   Lemma (nat_from_bytes_le b == nat_from_bytes_le (Seq.slice b 0 i) + pow2 (i * 8) * nat_from_bytes_le (Seq.slice b i len))
 
-val uints_from_bytes_le_nat_lemma: #t:inttype{~(t == U1)} -> #l:secrecy_level -> #len:size_nat{len * numbytes t < pow2 32}
+val uints_from_bytes_le_nat_lemma: #t:inttype{unsigned t /\ ~(U1? t)} -> #l:secrecy_level -> #len:size_nat{len * numbytes t < pow2 32}
   -> b:lbytes_l l (len * numbytes t) ->
   Lemma (nat_from_intseq_le (uints_from_bytes_le #t #l #len b) == nat_from_bytes_le b)
 
-val uints_to_bytes_le_nat_lemma: #t:inttype{~(t == U1)} -> #l:secrecy_level -> len:nat{len * numbytes t < pow2 32}
+val uints_to_bytes_le_nat_lemma: #t:inttype{unsigned t /\ ~(U1? t)} -> #l:secrecy_level -> len:nat{len * numbytes t < pow2 32}
   -> n:nat{n < pow2 (bits t * len)} ->
   Lemma (uints_to_bytes_le #t #l #len (nat_to_intseq_le #t #l len n) == nat_to_bytes_le (len * numbytes t) n)
 
 val nat_from_intseq_le_inj:
-  #t:inttype -> #l:secrecy_level -> b1:seq (uint_t t l) -> b2:seq (uint_t t l) ->
+  #t:inttype{unsigned t} -> #l:secrecy_level -> b1:seq (uint_t t l) -> b2:seq (uint_t t l) ->
   Lemma
     (requires length b1 == length b2 /\ nat_from_intseq_le b1 == nat_from_intseq_le b2)
     (ensures Seq.equal b1 b2)
     (decreases (length b1))
 
 val lemma_nat_to_from_bytes_be_preserves_value: #l:secrecy_level -> b:bytes_l l -> len:size_nat{len == length b} -> x:size_nat{x < pow2 (8 * len)} ->
-  Lemma
-  (requires (True))
-  (ensures  (nat_from_bytes_be (nat_to_bytes_be #l len x) == x))
+  Lemma (nat_from_bytes_be (nat_to_bytes_be #l len x) == x)
 
 val lemma_nat_to_from_bytes_le_preserves_value: #l:secrecy_level -> b:bytes_l l -> len:size_nat{len == length b} -> x:size_nat{x < pow2 (8 * len)} ->
-  Lemma
-  (requires (True))
-  (ensures  (nat_from_bytes_le (nat_to_bytes_le #l len x) == x))
+  Lemma (nat_from_bytes_le (nat_to_bytes_le #l len x) == x)
